src/tactics/FStar.Tactics.Basic.fsti
@@ -105,5 +105,5 @@ val t_commute_applied_match : unit -> tac unit
 
 val is_implicit_for_goal (g:goal) (i:TcComm.implicit) : bool
 val mark_implicit_as_allow_untyped (i:TcComm.implicit) : TcComm.implicit
-
+val goal_with_type : goal -> typ -> tac goal
 
