src/tactics/FStar.Tactics.Types.fsti
@@ -89,7 +89,7 @@ val set_ps_psc : Cfg.psc -> proofstate -> proofstate
 val goal_env: goal -> env
 val goal_witness: goal -> term
 val goal_type: goal -> term
-val goal_with_type: goal -> term -> goal
+val goal_with_type_pure: goal -> term -> goal
 val goal_with_env: goal -> env -> goal
 val is_guard : goal -> bool
 
